src/riot/asn1/ASN1.Spec.Value.OCTET_STRING.fst
@@ -37,32 +37,18 @@ module B32 = FStar.Bytes
 //////////////////////////////////////////////////////////
 
 /// Decodes input bytes into our representation of a OCTET_STRING value
-noextract
-let synth_asn1_octet_string
-  (l: asn1_value_length_of_type OCTET_STRING)
-  (s32: B32.lbytes l)
-: GTot (value: datatype_of_asn1_type OCTET_STRING{v (dfst value) == l})
+let synth_asn1_octet_string l s32
 = (|u l, s32|)
 
 
 /// Encodes our representation of a OCTET_STRING into bytes
-noextract
-let synth_asn1_octet_string_inverse
-  (l: asn1_value_length_of_type OCTET_STRING)
-  (value: datatype_of_asn1_type OCTET_STRING{v (dfst value) == l})
-: GTot (s32: B32.lbytes l{ value == synth_asn1_octet_string l s32 })
+let synth_asn1_octet_string_inverse l value
 = dsnd value
-
-inline_for_extraction noextract
-let parse_asn1_octet_string_kind (l: asn1_value_length_of_type OCTET_STRING) = total_constant_size_parser_kind l
 
 ///
 /// Parser
 ///
-noextract
-let parse_asn1_octet_string
-  (l: asn1_value_length_of_type OCTET_STRING)
-: parser (parse_asn1_octet_string_kind l) (x: datatype_of_asn1_type OCTET_STRING{v (dfst x) == l})
+let parse_asn1_octet_string l
 = parse_flbytes l
   `parse_synth`
   synth_asn1_octet_string l
@@ -70,10 +56,7 @@ let parse_asn1_octet_string
 ///
 /// Serializer
 ///
-noextract
-let serialize_asn1_octet_string
-  (l: asn1_value_length_of_type OCTET_STRING)
-: serializer (parse_asn1_octet_string l)
+let serialize_asn1_octet_string l
 = serialize_synth
   (* p1 *) (parse_flbytes l)
   (* f2 *) (synth_asn1_octet_string l)
@@ -87,28 +70,14 @@ let serialize_asn1_octet_string
 ///
 
 /// Reveal the computation of parse
-noextract
-let lemma_parse_asn1_octet_string_unfold
-  (l: asn1_value_length_of_type OCTET_STRING)
-  (input: bytes)
-: Lemma (
-  parse (parse_asn1_octet_string l) input ==
- (match parse (parse_flbytes l) input with
-  | None -> None
-  | Some (ls, consumed) -> Some (synth_asn1_octet_string l ls, consumed)))
+let lemma_parse_asn1_octet_string_unfold l input
 = parse_synth_eq
   (* p1 *) (parse_flbytes l)
   (* f2 *) (synth_asn1_octet_string l)
   (* in *) (input)
 
 /// Reveal the computation of serialize
-noextract
-let lemma_serialize_asn1_octet_string_unfold
-  (l: asn1_value_length_of_type OCTET_STRING)
-  (value: datatype_of_asn1_type OCTET_STRING{v (dfst value) == l})
-: Lemma (
-  serialize (serialize_asn1_octet_string l) value ==
-  serialize (serialize_flbytes l) (synth_asn1_octet_string_inverse l value))
+let lemma_serialize_asn1_octet_string_unfold l value
 = serialize_synth_eq
   (* p1 *) (parse_flbytes l)
   (* f2 *) (synth_asn1_octet_string l)
@@ -118,12 +87,7 @@ let lemma_serialize_asn1_octet_string_unfold
   (* in *) (value)
 
 /// Reveal the length of a serialzation
-noextract
-let lemma_serialize_asn1_octet_string_size
-  (l: asn1_value_length_of_type OCTET_STRING)
-  (value: datatype_of_asn1_type OCTET_STRING{v (dfst value) == l})
-: Lemma (
-  Seq.length (serialize (serialize_asn1_octet_string l) value) == l)
+let lemma_serialize_asn1_octet_string_size l value
 = parser_kind_prop_equiv (parse_asn1_octet_string_kind l) (parse_asn1_octet_string l);
   lemma_serialize_asn1_octet_string_unfold l value
 
@@ -133,20 +97,8 @@ let lemma_serialize_asn1_octet_string_size
 ///////////////////////////////////////////////////////////
 
 /// parser tag for the `tagged_union` combinators
-noextract
-let parser_tag_of_octet_string
-  (x: datatype_of_asn1_type OCTET_STRING)
-: GTot (the_asn1_tag OCTET_STRING & asn1_value_int32_of_type OCTET_STRING)
+let parser_tag_of_octet_string x
 = (OCTET_STRING, dfst x)
-
-inline_for_extraction noextract
-let parse_asn1_octet_string_TLV_kind
-: parser_kind
-= parse_asn1_tag_kind
-  `and_then_kind`
-  parse_asn1_length_kind_of_type OCTET_STRING
-  `and_then_kind`
-  weak_kind_of_type OCTET_STRING
 
 ///
 /// A pair of aux parser/serializer, which explicitly coerce the `OCTET_STRING` value
@@ -160,31 +112,20 @@ let parse_asn1_octet_string_TLV_kind
 /// Convert an `OCTET_STRING` value from the subtype used by its value parser to the subtype
 /// used by its TLV parser/serializer
 /// (value : subtype_{value}) <: subtype_{TLV}
-noextract
-let synth_asn1_octet_string_V
-  (tag: (the_asn1_tag OCTET_STRING & asn1_value_int32_of_type OCTET_STRING))
-  (value: datatype_of_asn1_type OCTET_STRING { v (dfst value) == v (snd tag) })
-: GTot (refine_with_tag parser_tag_of_octet_string tag)
+let synth_asn1_octet_string_V tag value
 = value
 
 /// Convert an `OCTET_STRING` value from the subtype used by its TLV parser to the subtype
 /// used by its value parser/serializer
 /// (value : subtype_{TLV}) <: subtype_{value}
-noextract
-let synth_asn1_octet_string_V_inverse
-  (tag: (the_asn1_tag OCTET_STRING & asn1_value_int32_of_type OCTET_STRING))
-  (value': refine_with_tag parser_tag_of_octet_string tag)
-: GTot (value: datatype_of_asn1_type OCTET_STRING { v (dfst value) == v (snd tag) /\ value' == synth_asn1_octet_string_V tag value})
+let synth_asn1_octet_string_V_inverse tag value'
 = value'
 
 
 ///
 /// Aux parser
 ///
-noextract
-let parse_asn1_octet_string_V
-  (tag: (the_asn1_tag OCTET_STRING & asn1_value_int32_of_type OCTET_STRING))
-: parser (weak_kind_of_type OCTET_STRING) (refine_with_tag parser_tag_of_octet_string tag)
+let parse_asn1_octet_string_V tag
 = weak_kind_of_type OCTET_STRING
   `weaken`
   parse_asn1_octet_string (v (snd tag))
@@ -194,10 +135,7 @@ let parse_asn1_octet_string_V
 ///
 /// Aux serializer
 ///
-noextract
-let serialize_asn1_octet_string_V
-  (tag: (the_asn1_tag OCTET_STRING & asn1_value_int32_of_type OCTET_STRING))
-: serializer (parse_asn1_octet_string_V tag)
+let serialize_asn1_octet_string_V tag
 = serialize_synth
   (* p1 *) (weak_kind_of_type OCTET_STRING
             `weaken`
@@ -214,15 +152,7 @@ let serialize_asn1_octet_string_V
 ///
 
 /// Reveal the computation of parse
-noextract
-let lemma_parse_asn1_octet_string_V_unfold
-  (tag: (the_asn1_tag OCTET_STRING & asn1_value_int32_of_type OCTET_STRING))
-  (input: bytes)
-: Lemma (
-  parse (parse_asn1_octet_string_V tag) input ==
- (match parse (parse_asn1_octet_string (v (snd tag))) input with
-  | None -> None
-  | Some (value, consumed) ->  Some (synth_asn1_octet_string_V tag value, consumed)))
+let lemma_parse_asn1_octet_string_V_unfold tag input
 = parse_synth_eq
   (* p1 *) (weak_kind_of_type OCTET_STRING
             `weaken`
@@ -256,9 +186,7 @@ let lemma_serialize_asn1_octet_string_V_unfold
 ///
 /// ASN1 `OCTET_STRING` TLV Parser
 ///
-noextract
 let parse_asn1_octet_string_TLV
-: parser parse_asn1_octet_string_TLV_kind (datatype_of_asn1_type OCTET_STRING)
 = parse_tagged_union
   (* pt *) (parse_asn1_tag_of_type OCTET_STRING
             `nondep_then`
@@ -269,9 +197,7 @@ let parse_asn1_octet_string_TLV
 ///
 /// Serializer
 ///
-noextract
 let serialize_asn1_octet_string_TLV
-: serializer parse_asn1_octet_string_TLV
 = serialize_tagged_union
   (* st *) (serialize_asn1_tag_of_type OCTET_STRING
             `serialize_nondep_then`
@@ -287,25 +213,7 @@ let serialize_asn1_octet_string_TLV
 #restart-solver
 #push-options "--z3rlimit 32 --initial_ifuel 8"
 noextract
-let lemma_parse_asn1_octet_string_TLV_unfold
-  (input: bytes)
-: Lemma (
-  parse parse_asn1_octet_string_TLV input ==
- (match parse (parse_asn1_tag_of_type OCTET_STRING) input with
-  | None -> None
-  | Some (tag, consumed_tag) ->
-    (let input_LV = Seq.slice input consumed_tag (Seq.length input) in
-     match parse (parse_asn1_length_of_type OCTET_STRING) input_LV with
-     | None -> None
-     | Some (len, consumed_len) ->
-       (let input_V = Seq.slice input_LV consumed_len (Seq.length input_LV) in
-        match parse (parse_asn1_octet_string_V (tag, len)) input_V with
-        | None -> None
-        | Some (value, consumed_value) ->
-               Some ((synth_asn1_octet_string_V (tag,len) value),
-                     (consumed_tag + consumed_len + consumed_value <: consumed_length input)))
-     ))
-)
+let lemma_parse_asn1_octet_string_TLV_unfold input
 = nondep_then_eq
   (* p1 *) (parse_asn1_tag_of_type OCTET_STRING)
   (* p2 *) (parse_asn1_length_of_type OCTET_STRING)
@@ -330,17 +238,7 @@ let lemma_parse_asn1_octet_string_TLV_unfold
 
 /// Reveal the computation of serialize
 #push-options "--z3rlimit 32"
-noextract
-let lemma_serialize_asn1_octet_string_TLV_unfold
-  (value: datatype_of_asn1_type OCTET_STRING)
-: Lemma (
-  serialize serialize_asn1_octet_string_TLV value ==
-  serialize (serialize_asn1_tag_of_type OCTET_STRING) OCTET_STRING
-  `Seq.append`
-  serialize (serialize_asn1_length_of_type OCTET_STRING) (dfst value)
-  `Seq.append`
-  serialize (serialize_asn1_octet_string (v (dfst value))) value
-)
+let lemma_serialize_asn1_octet_string_TLV_unfold value
 = serialize_nondep_then_eq
   (* s1 *) (serialize_asn1_tag_of_type OCTET_STRING)
   (* s2 *) (serialize_asn1_length_of_type OCTET_STRING)
@@ -357,17 +255,10 @@ let lemma_serialize_asn1_octet_string_TLV_unfold
 
 /// Reveal the size of a serialzation
 #push-options "--z3rlimit 16"
-noextract
-let lemma_serialize_asn1_octet_string_TLV_size
-  (value: datatype_of_asn1_type OCTET_STRING)
-: Lemma (
-  Seq.length (serialize serialize_asn1_octet_string_TLV value) ==
-  1 + length_of_asn1_length (dfst value) + B32.length (dsnd value)
-)
+let lemma_serialize_asn1_octet_string_TLV_size value
 = lemma_serialize_asn1_octet_string_TLV_unfold value;
   lemma_serialize_asn1_tag_of_type_size OCTET_STRING OCTET_STRING;
   lemma_serialize_asn1_length_size (dfst value);
   serialize_asn1_length_of_type_eq OCTET_STRING (dfst value);
   lemma_serialize_asn1_octet_string_size (v (dfst value)) value
 #pop-options
-
