src/riot/asn1/ASN1.Low.Value.OCTET_STRING.fsti
@@ -1,0 +1,18 @@
+module ASN1.Low.Value.OCTET_STRING
+
+open ASN1.Base
+open ASN1.Spec.Value.OCTET_STRING
+open ASN1.Low.Base
+
+open FStar.Integers
+
+(* NOTE: Read after `ASN1.Spec.Tag`, `ASN1.Spec.Length` *)
+
+inline_for_extraction
+val serialize32_asn1_octet_string_backwards
+  (len: asn1_value_int32_of_type OCTET_STRING)
+: (serializer32_backwards (serialize_asn1_octet_string (v len)))
+
+// inline_for_extraction
+val serialize32_asn1_octet_string_TLV_backwards (_:unit)
+: (serializer32_backwards serialize_asn1_octet_string_TLV)
