src/riot/asn1/ASN1.Spec.Value.OCTET_STRING.fsti
@@ -1,0 +1,225 @@
+module ASN1.Spec.Value.OCTET_STRING
+
+open ASN1.Spec.Base
+open LowParse.Spec.Bytes
+
+open ASN1.Base
+open ASN1.Spec.Tag
+open ASN1.Spec.Length
+
+open FStar.Integers
+
+module B32 = FStar.Bytes
+
+(* NOTE: Read after `ASN1.Spec.Tag`, `ASN1.Spec.Length`, `ASN1.Spec.Value.OCTET_STRING` *)
+
+(* NOTE: This module defines:
+         1) The ASN1 `OCTET_STRING` Value Parser and Serializer
+         2) The ASN1 `OCTET_STRING` TLV Parser and Serializer
+
+         And each part is organized as:
+         1) Aux (ghost) functions with prefix `filter_` to filter out invalid input bytes
+         2) Aux (ghost) functions with prefix `synth_` to decode the valid input bytes into our
+            representation of OCTET_STRING values. These functions are injective.
+         3) Aux (ghost) functions with prefix `synth_` and suffix `_inverse` to encode our
+            representation of OCTET_STRING into bytes. These functions are the inverse of
+            corresponding synth functions.
+         4) Functions with the prefix `parse_` are parsers constructed using parser combinators and
+            aux functions.
+         5) Functions with the prefix `serialize_` are serializers constructed using serializer
+            combinators and aux functions.
+         6) Lemma with suffix `_unfold` reveals the computation of parser/serialzier.
+         7) Lemma with suffix `_size` reveals the length of a serialization.
+*)
+
+///////////////////////////////////////////////////////////
+//// ASN1 `OCTET_STRING` Value Parser and Serializer
+//////////////////////////////////////////////////////////
+
+/// Decodes input bytes into our representation of a OCTET_STRING value
+noextract
+val synth_asn1_octet_string
+  (l: asn1_value_length_of_type OCTET_STRING)
+  (s32: B32.lbytes l)
+: GTot (value: datatype_of_asn1_type OCTET_STRING{v (dfst value) == l})
+
+
+/// Encodes our representation of a OCTET_STRING into bytes
+noextract
+val synth_asn1_octet_string_inverse
+  (l: asn1_value_length_of_type OCTET_STRING)
+  (value: datatype_of_asn1_type OCTET_STRING{v (dfst value) == l})
+: GTot (s32: B32.lbytes l{ value == synth_asn1_octet_string l s32 })
+
+inline_for_extraction noextract
+let parse_asn1_octet_string_kind (l: asn1_value_length_of_type OCTET_STRING) = total_constant_size_parser_kind l
+
+///
+/// Parser
+///
+val parse_asn1_octet_string
+  (l: asn1_value_length_of_type OCTET_STRING)
+: parser (parse_asn1_octet_string_kind l) (x: datatype_of_asn1_type OCTET_STRING{v (dfst x) == l})
+
+///
+/// Serializer
+///
+val serialize_asn1_octet_string
+  (l: asn1_value_length_of_type OCTET_STRING)
+: serializer (parse_asn1_octet_string l)
+
+
+///
+/// Lemmas
+///
+
+/// Reveal the computation of parse
+val lemma_parse_asn1_octet_string_unfold
+  (l: asn1_value_length_of_type OCTET_STRING)
+  (input: bytes)
+: Lemma (
+  parse (parse_asn1_octet_string l) input ==
+ (match parse (parse_flbytes l) input with
+  | None -> None
+  | Some (ls, consumed) -> Some (synth_asn1_octet_string l ls, consumed)))
+
+/// Reveal the computation of serialize
+val lemma_serialize_asn1_octet_string_unfold
+  (l: asn1_value_length_of_type OCTET_STRING)
+  (value: datatype_of_asn1_type OCTET_STRING{v (dfst value) == l})
+: Lemma (
+  serialize (serialize_asn1_octet_string l) value ==
+  serialize (serialize_flbytes l) (synth_asn1_octet_string_inverse l value))
+
+/// Reveal the length of a serialzation
+val lemma_serialize_asn1_octet_string_size
+  (l: asn1_value_length_of_type OCTET_STRING)
+  (value: datatype_of_asn1_type OCTET_STRING{v (dfst value) == l})
+: Lemma (
+  Seq.length (serialize (serialize_asn1_octet_string l) value) == l)
+
+
+///////////////////////////////////////////////////////////
+//// ASN1 `OCTET_STRING` TLV Parser and Serializer
+///////////////////////////////////////////////////////////
+
+/// parser tag for the `tagged_union` combinators
+
+noextract
+val parser_tag_of_octet_string
+  (x: datatype_of_asn1_type OCTET_STRING)
+: GTot (the_asn1_tag OCTET_STRING & asn1_value_int32_of_type OCTET_STRING)
+
+inline_for_extraction noextract
+let parse_asn1_octet_string_TLV_kind
+: parser_kind
+= parse_asn1_tag_kind
+  `and_then_kind`
+  parse_asn1_length_kind_of_type OCTET_STRING
+  `and_then_kind`
+  weak_kind_of_type OCTET_STRING
+
+///
+/// A pair of aux parser/serializer, which explicitly coerce the `OCTET_STRING` value
+/// between the subtype used by `OCTET_STRING` value parser/serialzier and `OCTET_STRING`
+/// TLV parser/serializer.
+///
+/// NOTE: I found that have this aux parser explicitly defined will make the prove of
+///       `_unfold` lemmas simpler.
+///
+
+/// Convert an `OCTET_STRING` value from the subtype used by its value parser to the subtype
+/// used by its TLV parser/serializer
+/// (value : subtype_{value}) <: subtype_{TLV}
+
+noextract
+val synth_asn1_octet_string_V
+  (tag: (the_asn1_tag OCTET_STRING & asn1_value_int32_of_type OCTET_STRING))
+  (value: datatype_of_asn1_type OCTET_STRING { v (dfst value) == v (snd tag) })
+: GTot (refine_with_tag parser_tag_of_octet_string tag)
+
+/// Convert an `OCTET_STRING` value from the subtype used by its TLV parser to the subtype
+/// used by its value parser/serializer
+/// (value : subtype_{TLV}) <: subtype_{value}
+
+noextract
+val synth_asn1_octet_string_V_inverse
+  (tag: (the_asn1_tag OCTET_STRING & asn1_value_int32_of_type OCTET_STRING))
+  (value': refine_with_tag parser_tag_of_octet_string tag)
+: GTot (value: datatype_of_asn1_type OCTET_STRING { v (dfst value) == v (snd tag) /\ value' == synth_asn1_octet_string_V tag value})
+
+
+///
+/// Aux parser
+///
+
+noextract
+val parse_asn1_octet_string_V
+  (tag: (the_asn1_tag OCTET_STRING & asn1_value_int32_of_type OCTET_STRING))
+: parser (weak_kind_of_type OCTET_STRING) (refine_with_tag parser_tag_of_octet_string tag)
+
+///
+/// Aux serializer
+///
+
+noextract
+val serialize_asn1_octet_string_V
+  (tag: (the_asn1_tag OCTET_STRING & asn1_value_int32_of_type OCTET_STRING))
+: serializer (parse_asn1_octet_string_V tag)
+
+///
+/// Lemmas
+///
+
+/// Reveal the computation of parse
+
+val lemma_parse_asn1_octet_string_V_unfold
+  (tag: (the_asn1_tag OCTET_STRING & asn1_value_int32_of_type OCTET_STRING))
+  (input: bytes)
+: Lemma (
+  parse (parse_asn1_octet_string_V tag) input ==
+ (match parse (parse_asn1_octet_string (v (snd tag))) input with
+  | None -> None
+  | Some (value, consumed) ->  Some (synth_asn1_octet_string_V tag value, consumed)))
+
+
+//////////////////////////////////////////////////////////
+///
+/// ASN1 `OCTET_STRING` TLV Parser
+///
+noextract
+val parse_asn1_octet_string_TLV
+: parser parse_asn1_octet_string_TLV_kind (datatype_of_asn1_type OCTET_STRING)
+
+///
+/// Serializer
+///
+noextract
+val serialize_asn1_octet_string_TLV
+: serializer parse_asn1_octet_string_TLV
+
+///
+/// Lemmas
+///
+
+/// Reveal the computation of serialize
+
+val lemma_serialize_asn1_octet_string_TLV_unfold
+  (value: datatype_of_asn1_type OCTET_STRING)
+: Lemma (
+  serialize serialize_asn1_octet_string_TLV value ==
+  serialize (serialize_asn1_tag_of_type OCTET_STRING) OCTET_STRING
+  `Seq.append`
+  serialize (serialize_asn1_length_of_type OCTET_STRING) (dfst value)
+  `Seq.append`
+  serialize (serialize_asn1_octet_string (v (dfst value))) value
+)
+
+/// Reveal the size of a serialzation
+
+val lemma_serialize_asn1_octet_string_TLV_size
+  (value: datatype_of_asn1_type OCTET_STRING)
+: Lemma (
+  Seq.length (serialize serialize_asn1_octet_string_TLV value) ==
+  1 + length_of_asn1_length (dfst value) + B32.length (dsnd value)
+)
